values.v
@@ -1,22 +1,23 @@
 (* Copyright (c) 2012-2013, Robbert Krebbers. *)
 (* This file is distributed under the terms of the BSD license. *)
 Require Export memory_values base_values.
+Local Open Scope ctype_scope.
 
 Inductive val (Ti Vi : Set) :=
   | VBase : base_val Ti Vi → val Ti Vi
-  | VArray : type Ti → list (val Ti Vi) → val Ti Vi
+  | VArray : list (val Ti Vi) → val Ti Vi
   | VStruct : tag → list (val Ti Vi) → val Ti Vi
   | VUnion : tag → nat → val Ti Vi → val Ti Vi
   | VUnionNone : tag → list (val Ti Vi) → val Ti Vi.
 Arguments VBase {_ _} _.
-Arguments VArray {_ _} _ _.
+Arguments VArray {_ _} _.
 Arguments VStruct {_ _} _ _.
 Arguments VUnion {_ _} _ _ _.
 Arguments VUnionNone  {_ _} _ _.
 
 Instance: Injective (=) (=) (@VBase Ti Vi).
 Proof. by injection 1. Qed.
-Instance: Injective (=) (=) (@VArray Ti Vi τ).
+Instance: Injective (=) (=) (@VArray Ti Vi).
 Proof. by injection 1. Qed.
 Instance: Injective (=) (=) (@VStruct Ti Vi s).
 Proof. by injection 1. Qed.
@@ -33,8 +34,7 @@ Proof.
   fix go v1 v2 : Decision (v1 = v2) :=
   match v1, v2 with
   | VBase v1, VBase v2 => cast_if (decide_rel (=) v1 v2)
-  | VArray τ1 vs1, VArray τ2 vs2 =>
-     cast_if_and (decide_rel (=) τ1 τ2) (decide_rel (=) vs1 vs2)
+  | VArray vs1, VArray vs2 => cast_if (decide_rel (=) vs1 vs2)
   | VStruct s1 vs1, VStruct s2 vs2 =>
      cast_if_and (decide_rel (=) s1 s2) (decide_rel (=) vs1 vs2)
   | VUnion s1 i1 v1, VUnion s2 i2 v2 =>
@@ -49,16 +49,15 @@ Defined.
 Section val_ind.
   Context {Ti Vi} (P : val Ti Vi → Prop).
   Context (Pbase : ∀ v, P (VBase v)).
-  Context (Parray : ∀ τ vs, Forall P vs → P (VArray τ vs)).
+  Context (Parray : ∀ vs, Forall P vs → P (VArray vs)).
   Context (Pstruct : ∀ s vs, Forall P vs → P (VStruct s vs)).
   Context (Punion : ∀ s i v, P v → P (VUnion s i v)).
   Context (Punion_none : ∀ s vs, Forall P vs → P (VUnionNone s vs)).
-
   Definition val_ind_alt: ∀ v, P v :=
     fix go v :=
     match v return P v with
     | VBase v => Pbase v
-    | VArray τ vs => Parray _ _ $ list_ind (Forall _)
+    | VArray vs => Parray _ $ list_ind (Forall _)
        (Forall_nil_2 _) (λ v _, Forall_cons_2 _ _ _ (go v)) vs
     | VStruct s vs => Pstruct _ _ $ list_ind (Forall _)
        (Forall_nil_2 _) (λ v _, Forall_cons_2 _ _ _ (go v)) vs
@@ -73,7 +72,7 @@ Definition val_map {Ti Vi} (f : base_val Ti Vi → base_val Ti Vi) :
   fix go v :=
   match v with
   | VBase v => VBase (f v)
-  | VArray τ vs => VArray τ (go <$> vs)
+  | VArray vs => VArray (go <$> vs)
   | VStruct s vs => VStruct s (go <$> vs)
   | VUnion s i v => VUnion s i (go v)
   | VUnionNone s vs => VUnionNone s (go <$> vs)
@@ -81,7 +80,7 @@ Definition val_map {Ti Vi} (f : base_val Ti Vi → base_val Ti Vi) :
 
 Inductive val_forall {Ti Vi} (P : base_val Ti Vi → Prop) : val Ti Vi → Prop :=
   | VBase_forall v : P v → val_forall P (VBase v)
-  | VArray_forall τ vs : Forall (val_forall P) vs → val_forall P (VArray τ vs)
+  | VArray_forall vs : Forall (val_forall P) vs → val_forall P (VArray vs)
   | VStruct_forall s vs : Forall (val_forall P) vs → val_forall P (VStruct s vs)
   | VUnion_forall s i v : val_forall P v → val_forall P (VUnion s i v)
   | VUnionNone_forall s vs :
@@ -91,19 +90,18 @@ Section val_forall_ind.
   Context {Ti Vi} (P : base_val Ti Vi → Prop).
   Context (Q : val Ti Vi → Prop).
   Context (Qbase : ∀ v, P v → Q (VBase v)).
-  Context (Qarray : ∀ τ vs,
-    Forall (val_forall P) vs → Forall Q vs → Q (VArray τ vs)).
+  Context (Qarray : ∀ vs,
+    Forall (val_forall P) vs → Forall Q vs → Q (VArray vs)).
   Context (Qstruct : ∀ s vs,
     Forall (val_forall P) vs → Forall Q vs → Q (VStruct s vs)).
   Context (Qunion : ∀ s i v, val_forall P v → Q v → Q (VUnion s i v)).
   Context (Qunion_none : ∀ s vs,
     Forall (val_forall P) vs → Forall Q vs → Q (VUnionNone s vs)).
-
   Definition val_forall_ind_alt: ∀ v, val_forall P v → Q v :=
     fix go v Hv :=
     match Hv in val_forall _ v return Q v with
     | VBase_forall _ H => Qbase _ H
-    | VArray_forall _ _ H => Qarray _ _ H (Forall_impl _ _ _ H go)
+    | VArray_forall _ H => Qarray _ H (Forall_impl _ _ _ H go)
     | VStruct_forall _ _ H => Qstruct _ _ H (Forall_impl _ _ _ H go)
     | VUnion_forall _ _ _  H => Qunion _ _ _ H (go _ H)
     | VUnionNone_forall _ _ H => Qunion_none _ _ H (Forall_impl _ _ _ H go)
@@ -113,22 +111,24 @@ End val_forall_ind.
 Section operations.
   Context `{EnvSpec Ti Vi} `{TypeOfIndex Ti M}.
 
-  Global Instance type_of_val: TypeOf (type Ti) (val Ti Vi) := λ v,
+  Global Instance type_of_val: TypeOf (type Ti) (val Ti Vi) :=
+    fix go v :=
     match v with
-    | VBase v => TBase (type_of v)
-    | VArray τ vs => TArray τ (length vs)
-    | VStruct s _ => TStruct s
-    | VUnion s _ _ => TUnion s
-    | VUnionNone s _ => TUnion s
+    | VBase v => base (type_of v)
+    | VArray [] => TVoid
+    | VArray (v :: vs) => go v.[length (v :: vs)]
+    | VStruct s _ => struct s
+    | VUnion s _ _ => union s
+    | VUnionNone s _ => union s
     end.
 
   Definition val_of_bytes : type Ti → list (byte Ti Vi) → val Ti Vi :=
     type_iter
     (*i TBase =>     *) (λ τ bs,
-      VBase $ base_val_of_bytes τ $ resize (size_of (TBase τ)) BUndef bs)
+      VBase $ base_val_of_bytes τ $ resize (size_of (base τ)) BUndef bs)
     (*i TVoid =>     *) (λ bs, VBase $ VUndef $ TInt $ TsInt)
     (*i TArray =>    *) (λ τ n rec bs,
-      VArray τ $ array_of_bytes rec τ n bs)
+      VArray $ array_of_bytes rec τ n bs)
     (*i TCompound => *) (λ c s τs rec bs,
       match c with
       | Struct => VStruct s $ struct_of_bytes rec τs bs
@@ -142,12 +142,12 @@ Section operations.
     fix go v :=
     match v with
     | MBase τ bs => VBase (base_val_of_bytes τ bs)
-    | MArray τ vs => VArray τ (go <$> vs)
+    | MArray vs => VArray (go <$> vs)
     | MStruct s vs => VStruct s (go <$> vs)
     | MUnion s i v => VUnion s i (go v)
-    | MUnionNone s bs => val_of_bytes (TUnion s) bs
+    | MUnionNone s bs => val_of_bytes (union s) bs
     end.
- 
+
   Definition union_to_bytes (f : val Ti Vi → listset (mval Ti Vi))
       (sz : nat) (vs : list (val Ti Vi)) : listset (list (byte Ti Vi)) :=
     filter (λ bs, vs = flip val_of_bytes bs ∘ type_of <$> vs) $
@@ -157,17 +157,46 @@ Section operations.
     fix go v :=
     match v with
     | VBase v => MBase (type_of v) <$> base_val_to_bytes v
-    | VArray τ vs => MArray τ <$> mapM go vs
+    | VArray vs => MArray <$> mapM go vs
     | VStruct s vs => MStruct s <$> mapM go vs
     | VUnion s i v => MUnion s i <$> go v
     | VUnionNone s vs =>
-       MUnionNone s <$> union_to_bytes go (size_of (TUnion s)) vs
+       MUnionNone s <$> union_to_bytes go (size_of (union s)) vs
     end.
-    
+
+  Global Instance vtype_check: TypeCheck M (type Ti) (val Ti Vi) := λ m,
+    fix go v :=
+    match v with
+    | VBase v => TBase <$> type_check m v
+    | VArray [] => None
+    | VArray (v :: vs) =>
+       τ ← go v;
+       τs ← mapM go vs;
+       guard (Forall (= τ) τs);
+       Some (τ.[length (v :: vs)])
+    | VStruct s vs =>
+       τs ← get_env !! s;
+       τs' ← mapM go vs;
+       guard (τs = τs');
+       Some (struct s)
+    | VUnion s i v =>
+       τ ← get_env !! s ≫= (!! i);
+       τ' ← go v;
+       guard (τ = τ');
+       Some (union s)
+    | VUnionNone s vs =>
+       τs ← get_env !! s;
+       guard (1 ≠ length τs);
+       τs' ← mapM go vs;
+       guard (τs = τs');
+       _ ← choose (union_to_bytes mval_of_val (size_of (union s)) vs);
+       Some (union s)
+    end.
+
   Global Instance val_lookup_item:
       Lookup ref_seg (val Ti Vi) (val Ti Vi) := λ rs v,
     match rs, v with
-    | RArray i n _, VArray _ vs => guard (n = length vs); vs !! i
+    | RArray i n _, VArray vs => guard (n = length vs); vs !! i
     | RStruct i, VStruct _ vs => vs !! i
     | RUnion i _, VUnion s j v => guard (i = j); Some v
     | RUnion i _, VUnionNone s vs => vs !! i
@@ -187,97 +216,142 @@ Section vtyped.
   Inductive vtyped' (m : M) : val Ti Vi → type Ti → Prop :=
     | VBase_typed' v τ :
        m ⊢ v : τ →
-       vtyped' m (VBase v) (TBase τ)
-    | VArray_typed' vs τ n :
-       type_valid get_env τ →
-       n = length vs →
+       vtyped' m (VBase v) (base τ)
+    | VArray_typed' vs τ :
        Forall (λ v, vtyped' m v τ) vs →
-       vtyped' m (VArray τ vs) (TArray τ n)
+       length vs ≠ 0 →
+       vtyped' m (VArray vs) (τ.[length vs])
     | VStruct_typed' s vs τs :
        get_env !! s = Some τs →
        Forall2 (vtyped' m) vs τs →
-       vtyped' m (VStruct s vs) (TStruct s)
+       vtyped' m (VStruct s vs) (struct s)
     | VUnion_typed' s i τs v τ :
        get_env !! s = Some τs →
        τs !! i = Some τ →
        vtyped' m v τ →
-       vtyped' m (VUnion s i v) (TUnion s)
+       vtyped' m (VUnion s i v) (union s)
     | VUnionNone_typed' s vs τs bs :
        get_env !! s = Some τs →
        length τs ≠ 1 →
        Forall2 (vtyped' m) vs τs →
        vs = flip val_of_bytes bs <$> τs →
        Forall (byte_valid m) bs →
-       vtyped' m (VUnionNone s vs) (TUnion s).
+       vtyped' m (VUnionNone s vs) (union s).
   Global Instance vtyped: Typed M (type Ti) (val Ti Vi) := vtyped'.
 
-  Lemma VBase_typed m v τ : m ⊢ v : τ → m ⊢ VBase v : TBase τ.
+  Lemma val_of_bytes_base τ bs :
+    val_of_bytes (base τ) bs =
+      VBase $ base_val_of_bytes τ $ resize (size_of (base τ)) BUndef bs.
+  Proof. unfold val_of_bytes. by rewrite type_iter_base. Qed. 
+  Lemma val_of_bytes_array τ n bs :
+    val_of_bytes (τ.[n]) bs = VArray $ array_of_bytes (val_of_bytes τ) τ n bs.
+  Proof. unfold val_of_bytes. by rewrite type_iter_array. Qed.
+  Lemma val_of_bytes_compound c s τs bs :
+    get_env !! s = Some τs →
+    val_of_bytes (compound@{c} s) bs =
+      match c with
+      | Struct => VStruct s $ struct_of_bytes val_of_bytes τs bs
+      | Union =>
+         match list_singleton_dec τs with
+         | inleft (τ↾_) => VUnion s 0 $ val_of_bytes τ bs
+         | _ => VUnionNone s $ flip val_of_bytes bs <$> τs
+         end
+      end.
+  Proof.
+    intros Hs. unfold val_of_bytes. erewrite (type_iter_compound
+      (pointwise_relation (list (byte Ti Vi)) (@eq (val Ti Vi)))); eauto.
+    { clear s τs Hs bs. intros τ n f g Hfg bs. f_equal.
+      auto using array_of_bytes_ext. }
+    clear s τs Hs bs. intros f g [] s τs Hs Hτs bs.
+    { f_equal. auto using struct_of_bytes_ext. }
+    destruct (list_singleton_dec _) as [[??]|?]; subst; f_equal.
+    * by decompose_Forall.
+    * apply Forall_fmap_ext. eauto using Forall_impl.
+  Qed.
+
+  Lemma VBase_typed m v τ : m ⊢ v : τ → m ⊢ VBase v : base τ.
   Proof. by constructor. Qed.
   Lemma VArray_typed m vs τ n :
-    type_valid get_env τ → n = length vs →
-    m ⊢* vs : τ → m ⊢ VArray τ vs : TArray τ n.
-  Proof. by constructor. Qed.
+    n = length vs → m ⊢* vs : τ → n ≠ 0 → m ⊢ VArray vs : τ.[n].
+  Proof. intros; subst. by constructor. Qed.
   Lemma VStruct_typed m s vs τs :
-    get_env !! s = Some τs → m ⊢* vs :* τs → m ⊢ VStruct s vs : TStruct s.
+    get_env !! s = Some τs → m ⊢* vs :* τs → m ⊢ VStruct s vs : struct s.
   Proof. econstructor; eauto. Qed.
   Lemma VUnion_typed m s i τs v τ :
     get_env !! s = Some τs → τs !! i = Some τ →
-    m ⊢ v : τ → m ⊢ VUnion s i v : TUnion s.
+    m ⊢ v : τ → m ⊢ VUnion s i v : union s.
   Proof. econstructor; eauto. Qed.
+  Lemma val_of_bytes_typed m τ bs :
+    type_valid get_env τ → Forall (byte_valid m) bs → m ⊢ val_of_bytes τ bs : τ.
+  Proof.
+    intros Hτ. revert τ Hτ bs. refine (type_env_ind _ _ _ _).
+    * intros τ Hτ bs Hbs. rewrite val_of_bytes_base. apply VBase_typed;
+        auto using base_val_of_bytes_typed, Forall_resize, BUndef_valid.
+    * intros τ n Hτ IH ? bs Hbs. rewrite val_of_bytes_array. apply VArray_typed;
+        eauto using array_of_bytes_length, Forall_array_of_bytes_alt.
+    * intros [] s τs Hs Hτs IH _ bs Hbs.
+      { erewrite val_of_bytes_compound by eauto.
+        apply VStruct_typed with τs; eauto using Forall2_struct_of_bytes_alt. }
+      erewrite val_of_bytes_compound by eauto.
+      destruct (list_singleton_dec _) as [[τ ?]|Hτs_len]; subst.
+      + rewrite Forall_singleton in IH. eapply VUnion_typed, IH; eauto.
+      + apply VUnionNone_typed' with τs bs; auto using resize_length.
+        change (vtyped' m) with (typed m).
+        clear Hτs Hs Hτs_len; induction IH; simpl; constructor; auto.
+  Qed.
   Lemma VUnionNone_typed m s vs τs bs :
-    get_env !! s = Some τs → length τs ≠ 1 → m ⊢* vs :* τs →
-    vs = flip val_of_bytes bs <$> τs → Forall (byte_valid m) bs →
-    m ⊢ VUnionNone s vs : TUnion s.
-  Proof. econstructor; eauto. Qed.
+    get_env !! s = Some τs → length τs ≠ 1 →
+    vs = flip val_of_bytes bs <$> τs →
+    Forall (byte_valid m) bs → m ⊢ VUnionNone s vs : union s.
+  Proof.
+    intros Hs Hτs_len Hvs Hbs. subst.
+    eapply VUnionNone_typed'; eauto. change (vtyped' m) with (typed m).
+    elim (env_valid_lookup s τs Hs); simpl;
+      constructor; eauto using val_of_bytes_typed.
+  Qed.
 
   Lemma vtyped_inv_l m (P : type Ti → Prop) v τ :
     m ⊢ v : τ →
     match v with
-    | VBase v => (∀ τ', m ⊢ v : τ' → P (TBase τ')) → P τ
-    | VArray τ' vs =>
-       (∀ n, type_valid get_env τ' → n = length vs →
-         m ⊢* vs : τ' → P (TArray τ' n)) →
-       P τ
+    | VBase v => (∀ τ', m ⊢ v : τ' → P (base τ')) → P τ
+    | VArray vs =>
+       (∀ τ' n, n = length vs → m ⊢* vs : τ' → n ≠ 0 → P (τ'.[n])) → P τ
     | VStruct s vs =>
-       (∀ τs, get_env !! s = Some τs → m ⊢* vs :* τs → P (TStruct s)) →
-       P τ
+       (∀ τs, get_env !! s = Some τs → m ⊢* vs :* τs → P (struct s)) → P τ
     | VUnion s i v =>
        (∀ τs τ', get_env !! s = Some τs → τs !! i = Some τ' →
-         m ⊢ v : τ' → P (TUnion s)) →
-       P τ
+         m ⊢ v : τ' → P (union s)) → P τ
     | VUnionNone s vs =>
        (∀ τs bs,
          get_env !! s = Some τs → length τs ≠ 1 → m ⊢* vs :* τs →
          vs = flip val_of_bytes bs <$> τs → Forall (byte_valid m) bs →
-         P (TUnion s)) →
-       P τ
+         P (union s)) → P τ
     end.
   Proof. destruct 1; eauto. Qed.
 
   Section vtyped_ind.
     Context (m : M) (P : val Ti Vi → type Ti → Prop).
-    Context (Pbase : ∀ v τ, m ⊢ v : τ → P (VBase v) (TBase τ)).
-    Context (Parray : ∀ vs τ n,
-      type_valid get_env τ → n = length vs → m ⊢* vs : τ →
-      Forall (λ v, P v τ) vs → P (VArray τ vs) (TArray τ n)).
+    Context (Pbase : ∀ v τ, m ⊢ v : τ → P (VBase v) (base τ)).
+    Context (Parray : ∀ vs τ,
+      m ⊢* vs : τ → Forall (λ v, P v τ) vs →
+      length vs ≠ 0 → P (VArray vs) (τ.[length vs])).
     Context (Pstruct : ∀ s vs τs,
       get_env !! s = Some τs → m ⊢* vs :* τs → Forall2 P vs τs →
-      P (VStruct s vs) (TStruct s)).
+      P (VStruct s vs) (struct s)).
     Context (PUnion : ∀ s i τs v τ,
       get_env !! s = Some τs → τs !! i = Some τ → m ⊢ v : τ → P v τ →
-      P (VUnion s i v) (TUnion s)).
+      P (VUnion s i v) (union s)).
     Context (Punion_none : ∀ s vs τs bs,
       get_env !! s = Some τs → length τs ≠ 1 → m ⊢* vs :* τs →
       Forall2 P vs τs → vs = flip val_of_bytes bs <$> τs →
-      Forall (byte_valid m) bs → P (VUnionNone s vs) (TUnion s)).
-
+      Forall (byte_valid m) bs → P (VUnionNone s vs) (union s)).
     Lemma vtyped_ind : ∀ v τ, vtyped' m v τ → P v τ.
     Proof.
      exact (fix go v τ H :=
       match H in vtyped' _ v τ return P v τ with
       | VBase_typed' _ _ H => Pbase _ _ H
-      | VArray_typed' _ _ _ Hτ Hn H =>
-         Parray _ _ _ Hτ Hn H (Forall_impl _ _ _ H (λ v, go _ _))
+      | VArray_typed' _ _ Hvs Hn =>
+         Parray _ _ Hvs (Forall_impl _ _ _ Hvs (λ v, go _ _)) Hn
       | VStruct_typed' s _ _ Hs H =>
          Pstruct _ _ _ Hs H (Forall2_impl _ _ _ _ H go)
       | VUnion_typed' _ _ _ _ _ Hs Hτs H => PUnion _ _ _ _ _ Hs Hτs H (go _ _ H)
@@ -289,20 +363,18 @@ Section vtyped.
 
   Section vtyped_case.
     Context (m : M) (P : val Ti Vi → type Ti → Prop).
-    Context (Pbase : ∀ v τ, m ⊢ v : τ → P (VBase v) (TBase τ)).
-    Context (Parray : ∀ vs τ n,
-      type_valid get_env τ → n = length vs →
-      m ⊢* vs : τ → P (VArray τ vs) (TArray τ n)).
+    Context (Pbase : ∀ v τ, m ⊢ v : τ → P (VBase v) (base τ)).
+    Context (Parray : ∀ vs τ,
+      m ⊢* vs : τ → length vs ≠ 0 → P (VArray vs) (τ.[length vs])).
     Context (Pstruct : ∀ s vs τs,
-      get_env !! s = Some τs → m ⊢* vs :* τs → P (VStruct s vs) (TStruct s)).
+      get_env !! s = Some τs → m ⊢* vs :* τs → P (VStruct s vs) (struct s)).
     Context (PUnion : ∀ s i τs v τ,
       get_env !! s = Some τs → τs !! i = Some τ →
-      m ⊢ v : τ → P (VUnion s i v) (TUnion s)).
+      m ⊢ v : τ → P (VUnion s i v) (union s)).
     Context (Punion_none : ∀ s vs τs bs,
       get_env !! s = Some τs → length τs ≠ 1 → m ⊢* vs :* τs →
       vs = flip val_of_bytes bs <$> τs → Forall (byte_valid m) bs →
-      P (VUnionNone s vs) (TUnion s)).
-
+      P (VUnionNone s vs) (union s)).
     Lemma vtyped_case : ∀ v τ, vtyped' m v τ → P v τ.
     Proof. destruct 1; eauto. Qed.
   End vtyped_case.
@@ -316,16 +388,14 @@ Section val_le.
   Context `{EnvSpec Ti Vi} `{TypeOfIndex Ti M}.
 
   Inductive val_le' (m : M) : relation (val Ti Vi) :=
-    | VBase_le' v1 v2 :
-       v1 ⊑@{m} v2 → val_le' m (VBase v1) (VBase v2)
-    | VArray_le' vs1 vs2 τ :
-       Forall2 (val_le' m) vs1 vs2 → val_le' m (VArray τ vs1) (VArray τ vs2)
+    | VBase_le' v1 v2 : v1 ⊑@{m} v2 → val_le' m (VBase v1) (VBase v2)
+    | VArray_le' vs1 vs2 :
+       Forall2 (val_le' m) vs1 vs2 → val_le' m (VArray vs1) (VArray vs2)
     | VStruct_le' s vs1 vs2 :
        Forall2 (val_le' m) vs1 vs2 → val_le' m (VStruct s vs1) (VStruct s vs2)
     | VUnion_le' s i v1 v2 :
        val_le' m v1 v2 → val_le' m (VUnion s i v1) (VUnion s i v2)
-    | VUnionNone_le_refl' s vs :
-       val_le' m (VUnionNone s vs) (VUnionNone s vs)
+    | VUnionNone_le_refl' s vs : val_le' m (VUnionNone s vs) (VUnionNone s vs)
     | VUnionNone_le' s vs1 vs2 τs bs1 bs2 :
        get_env !! s = Some τs →
        vs1 = flip val_of_bytes bs1 <$> τs →
@@ -345,8 +415,7 @@ Section val_le.
 
   Lemma VBase_le m v1 v2 : v1 ⊑@{m} v2 → VBase v1 ⊑@{m} VBase v2.
   Proof. by constructor. Qed.
-  Lemma VArray_le m vs1 vs2 τ :
-    vs1 ⊑@{m}* vs2 → VArray τ vs1 ⊑@{m} VArray τ vs2.
+  Lemma VArray_le m vs1 vs2 : vs1 ⊑@{m}* vs2 → VArray vs1 ⊑@{m} VArray vs2.
   Proof. by constructor. Qed.
   Lemma VStruct_le m s vs1 vs2 :
     vs1 ⊑@{m}* vs2 → VStruct s vs1 ⊑@{m} VStruct s vs2.
@@ -372,11 +441,35 @@ Section val_le.
     VUnion s i v1 ⊑@{m} VUnionNone s vs2.
   Proof. econstructor; eauto. Qed.
 
+  Lemma val_of_bytes_le m τ bs1 bs2 :
+    type_valid get_env τ →
+    Forall (byte_valid m) bs1 → bs1 ⊑@{m}* bs2 →
+    val_of_bytes τ bs1 ⊑@{m} val_of_bytes τ bs2.
+  Proof.
+    intros Hτ. revert τ Hτ bs1 bs2. refine (type_env_ind _ _ _ _).
+    * intros τ ? bs1 bs2 Hbs. rewrite !val_of_bytes_base. constructor.
+      apply base_val_of_bytes_le;
+        auto using Forall_resize, BUndef_valid, Forall2_resize.
+    * intros τ n ? IH _ bs1 bs2 Hbs1 Hbs.
+      rewrite !val_of_bytes_array. apply VArray_le. revert bs1 bs2 Hbs1 Hbs.
+      induction n; simpl; auto using Forall2_take, Forall2_drop, Forall_drop.
+    * intros [] s τs Hs Hτs IH _ bs1 bs2 Hbs1 Hbs.
+      { erewrite !val_of_bytes_compound by eauto. apply VStruct_le.
+        clear Hs Hτs. unfold struct_of_bytes. revert bs1 bs2 Hbs1 Hbs.
+        induction (struct_fields_same_length τs);
+          intros; decompose_Forall; simpl;
+          auto using Forall2_take, Forall2_drop, Forall_drop. }
+      erewrite !val_of_bytes_compound by eauto.
+      destruct (list_singleton_dec _) as [[??]|?]; subst.
+      { rewrite Forall_singleton in IH. apply VUnion_le. auto. }
+      simpl. eapply VUnionNone_le; eauto.
+  Qed.
+
   Lemma val_le_inv_l m (P : val Ti Vi → Prop) v1 v2 :
     v1 ⊑@{m} v2 →
     match v1 with
     | VBase v1 => (∀ v2, v1 ⊑@{m} v2 → P (VBase v2)) → P v2
-    | VArray τ vs1 => (∀ vs2, vs1 ⊑@{m}* vs2 → P (VArray τ vs2)) → P v2
+    | VArray vs1 => (∀ vs2, vs1 ⊑@{m}* vs2 → P (VArray vs2)) → P v2
     | VStruct s vs1 => (∀ vs2, vs1 ⊑@{m}* vs2 → P (VStruct s vs2)) → P v2 
     | VUnion s i v1 =>
        (∀ v2, v1 ⊑@{m} v2 → P (VUnion s i v2)) →
@@ -406,7 +499,7 @@ Section val_le.
     v1 ⊑@{m} v2 →
     match v1, v2 with
     | VBase v1, VBase v2 => (v1 ⊑@{m} v2 → P) → P
-    | VArray τ1 vs1, VArray τ2 vs2 => (τ1 = τ2 → vs1 ⊑@{m}* vs2 → P) → P
+    | VArray vs1, VArray vs2 => (vs1 ⊑@{m}* vs2 → P) → P
     | VStruct s1 vs1, VStruct s2 vs2 => (s1 = s2 → vs1 ⊑@{m}* vs2 → P) → P 
     | VUnion s1 i1 v1, VUnion s2 i2 v2 =>
        (s1 = s2 → i1 = i2 → v1 ⊑@{m} v2 → P) → P
@@ -436,66 +529,11 @@ Section val_le.
     end.
   Proof. destruct 1; eauto. Qed.
 
-  Lemma val_of_bytes_base τ bs :
-    val_of_bytes (TBase τ) bs =
-      VBase $ base_val_of_bytes τ $ resize (size_of (TBase τ)) BUndef bs.
-  Proof. unfold val_of_bytes. by rewrite type_iter_base. Qed. 
-  Lemma val_of_bytes_array τ n bs :
-    val_of_bytes (TArray τ n) bs =
-      VArray τ $ array_of_bytes (val_of_bytes τ) τ n bs.
-  Proof. unfold val_of_bytes. by rewrite type_iter_array. Qed.
-  Lemma val_of_bytes_compound c s τs bs :
-    get_env !! s = Some τs →
-    val_of_bytes (TCompound c s) bs =
-      match c with
-      | Struct => VStruct s $ struct_of_bytes val_of_bytes τs bs
-      | Union =>
-         match list_singleton_dec τs with
-         | inleft (τ↾_) => VUnion s 0 $ val_of_bytes τ bs
-         | _ => VUnionNone s $ flip val_of_bytes bs <$> τs
-         end
-      end.
-  Proof.
-    intros Hs. unfold val_of_bytes. erewrite (type_iter_compound
-      (pointwise_relation (list (byte Ti Vi)) (@eq (val Ti Vi)))); eauto.
-    { clear s τs Hs bs. intros τ n f g Hfg bs. f_equal.
-      auto using array_of_bytes_ext. }
-    clear s τs Hs bs. intros f g [] s τs Hs Hτs bs.
-    { f_equal. auto using struct_of_bytes_ext. }
-    destruct (list_singleton_dec _) as [[??]|?]; subst; f_equal.
-    * by decompose_Forall.
-    * apply Forall_fmap_ext. eauto using Forall_impl.
-  Qed.
-
-  Lemma val_of_bytes_le m τ bs1 bs2 :
-    type_valid get_env τ →
-    Forall (byte_valid m) bs1 → bs1 ⊑@{m}* bs2 →
-    val_of_bytes τ bs1 ⊑@{m} val_of_bytes τ bs2.
-  Proof.
-    intros Hτ. revert τ Hτ bs1 bs2. refine (type_env_ind _ _ _ _).
-    * intros τ ? bs1 bs2 Hbs. rewrite !val_of_bytes_base. constructor.
-      apply base_val_of_bytes_le;
-        auto using Forall_resize, BUndef_valid, Forall2_resize.
-    * intros τ n ? IH bs1 bs2 Hbs1 Hbs.
-      rewrite !val_of_bytes_array. apply VArray_le. revert bs1 bs2 Hbs1 Hbs.
-      induction n; simpl; auto using Forall2_take, Forall2_drop, Forall_drop.
-    * intros [] s τs Hs Hτs IH bs1 bs2 Hbs1 Hbs.
-      { erewrite !val_of_bytes_compound by eauto. apply VStruct_le.
-        clear Hs Hτs. unfold struct_of_bytes. revert bs1 bs2 Hbs1 Hbs.
-        induction (struct_fields_same_length τs);
-          intros; decompose_Forall; simpl;
-          auto using Forall2_take, Forall2_drop, Forall_drop. }
-      erewrite !val_of_bytes_compound by eauto.
-      destruct (list_singleton_dec _) as [[??]|?]; subst.
-      { rewrite Forall_singleton in IH. apply VUnion_le. auto. }
-      simpl. eapply VUnionNone_le; eauto.
-  Qed.
-
   Section val_le_ind.
     Context (m : M) (P : val Ti Vi → val Ti Vi → Prop).
     Context (Pbase : ∀ v1 v2, v1 ⊑@{m} v2 → P (VBase v1) (VBase v2)).
-    Context (Parray : ∀ vs1 vs2 τ,
-      vs1 ⊑@{m}* vs2 → Forall2 P vs1 vs2 → P (VArray τ vs1) (VArray τ vs2)).
+    Context (Parray : ∀ vs1 vs2,
+      vs1 ⊑@{m}* vs2 → Forall2 P vs1 vs2 → P (VArray vs1) (VArray vs2)).
     Context (Pstruct : ∀ s vs1 vs2,
       vs1 ⊑@{m}* vs2 → Forall2 P vs1 vs2 → P (VStruct s vs1) (VStruct s vs2)).
     Context (Punion : ∀ s i v1 v2,
@@ -519,7 +557,6 @@ Section val_le.
       vs2 = flip val_of_bytes bs2 <$> τs →
       Forall (byte_valid m) bs2 →
       P (VUnion s i v1) (VUnionNone s vs2)).
-
     Lemma val_le_ind: ∀ v1 v2, val_le' m v1 v2 → P v1 v2.
     Proof.
      assert (∀ vs1 vs2,
@@ -545,7 +582,7 @@ Ltac val_le_constructor := first
 
 Inductive union_free `{EnvSpec Ti Vi} : val Ti Vi → Prop :=
   | VBase_union_free v : union_free (VBase v)
-  | VArray_union_free vs τ : Forall union_free vs → union_free (VArray τ vs)
+  | VArray_union_free vs : Forall union_free vs → union_free (VArray vs)
   | VStruct_union_free s vs : Forall union_free vs → union_free (VStruct s vs)
   | VUnion_union_free s v τ :
      get_env !! s = Some [τ] → union_free v → union_free (VUnion s 0 v)
@@ -555,27 +592,49 @@ Inductive union_free `{EnvSpec Ti Vi} : val Ti Vi → Prop :=
 Section union_free_ind.
   Context `{EnvSpec Ti Vi} (P : val Ti Vi → Prop).
   Context (Pbase : ∀ v, P (VBase v)).
-  Context (Parray : ∀ τ vs,
-    Forall union_free vs → Forall P vs → P (VArray τ vs)).
+  Context (Parray : ∀ vs,
+    Forall union_free vs → Forall P vs → P (VArray vs)).
   Context (Pstruct : ∀ s vs,
     Forall union_free vs → Forall P vs → P (VStruct s vs)).
   Context (Punion : ∀ s v τ,
     get_env !! s = Some [τ] → union_free v → P v → P (VUnion s 0 v)).
   Context (Punion_none : ∀ s vs,
     Forall union_free vs → Forall P vs → P (VUnionNone s vs)).
-
   Lemma union_free_ind_alt: ∀ v, union_free v → P v.
   Proof.
    exact (
     fix go v Hv :=
     match Hv in union_free v return P v with
     | VBase_union_free _ => Pbase _
-    | VArray_union_free _ _ H => Parray _ _ H (Forall_impl _ _ _ H go)
+    | VArray_union_free _ H => Parray _ H (Forall_impl _ _ _ H go)
     | VStruct_union_free _ _ H => Pstruct _ _ H (Forall_impl _ _ _ H go)
     | VUnion_union_free _ _ _ Hs H => Punion _ _ _ Hs H (go _ H)
     | VUnionNone_union_free _ _ H => Punion_none _ _ H (Forall_impl _ _ _ H go)
     end).
   Qed.
+  Global Instance union_free_dec: ∀ v, Decision (union_free v).
+   refine (
+    fix go v :=
+    match v return Decision (union_free v) with
+    | VBase v => left _
+    | VArray vs => cast_if (decide (Forall union_free vs))
+    | VStruct _ vs => cast_if (decide (Forall union_free vs))
+    | VUnion s i v =>
+       if decide (i = 0) then
+         match Some_dec (get_env !! s) with
+         | inleft(τs↾_) =>
+           match list_singleton_dec τs with
+           | inleft (_↾_) => cast_if (decide (union_free v))
+           | inright _ => right _
+           end
+         | _ => right _
+         end
+       else right _
+    | VUnionNone _ vs => cast_if (decide (Forall union_free vs))
+    end); first
+      [ subst; econstructor; eauto
+      | by inversion 1; simplify_option_equality].
+  Defined.
 End union_free_ind.
 
 Section val.
@@ -591,40 +650,23 @@ Implicit Types bs : list (byte Ti Vi).
 Implicit Types r : ref.
 Implicit Types rs : ref_seg.
 Context `{PropHolds (∀ m i τ,
-  type_of_index m i = Some τ → τ = TVoid ∨ type_valid get_env τ)}.
+  type_of_index m i = Some τ → type_valid get_env τ)}.
 
 Lemma vtyped_type_valid m v τ : m ⊢ v : τ → type_valid get_env τ.
 Proof.
-  induction 1 using @vtyped_ind;
-    econstructor; eauto using base_typed_type_valid.
+  induction 1 using @vtyped_ind; econstructor;
+    decompose_Forall_hyps; eauto using base_typed_type_valid.
 Qed.
 Global Instance: TypeOfSpec M (type Ti) (val Ti Vi).
-Proof. destruct 1; simpl; f_equal; eauto. eapply type_of_correct; eauto. Qed.
-
-Lemma val_of_bytes_typed m τ bs :
-  type_valid get_env τ → Forall (byte_valid m) bs → m ⊢ val_of_bytes τ bs : τ.
 Proof.
-  intros Hτ. revert τ Hτ bs. refine (type_env_ind _ _ _ _).
-  * intros τ Hτ bs Hbs. rewrite val_of_bytes_base.
-    vtyped_constructor; auto using base_val_of_bytes_typed,
-      Forall_resize, BUndef_valid.
-  * intros τ n Hτ IH bs Hbs. rewrite val_of_bytes_array. vtyped_constructor;
-      eauto using array_of_bytes_length, Forall_array_of_bytes_alt.
-  * intros [] s τs Hs Hτs IH bs Hbs.
-    { erewrite val_of_bytes_compound by eauto.
-      apply VStruct_typed with τs; eauto using Forall2_struct_of_bytes_alt. }
-    erewrite val_of_bytes_compound by eauto.
-    destruct (list_singleton_dec _) as [[τ ?]|Hτs_len]; subst.
-    + rewrite Forall_singleton in IH. eapply VUnion_typed, IH; eauto.
-    + apply VUnionNone_typed with τs bs;
-        auto using resize_length;
-        clear Hτs Hs Hτs_len; induction IH; simpl; constructor; auto.
+  induction 1 using @vtyped_ind; decompose_Forall_hyps; simpl; f_equal; eauto.
+  eapply type_of_correct; eauto.
 Qed.
-Lemma Forall_val_of_bytes_typed m τs bs :
+
+Lemma fmap_val_of_bytes_typed m τs bs :
   Forall (type_valid get_env) τs → Forall (byte_valid m) bs →
   m ⊢* (flip val_of_bytes bs <$> τs) :* τs.
 Proof. intros Hτs Hbs. induction Hτs; simpl; auto using val_of_bytes_typed. Qed.
-
 Lemma val_of_bytes_type_of m τ bs :
   type_valid get_env τ → Forall (byte_valid m) bs →
   type_of (val_of_bytes τ bs) = τ.
@@ -632,9 +674,7 @@ Proof. intros. eapply type_of_correct, val_of_bytes_typed; eauto. Qed.
 Lemma val_of_bytes_fmap_type_of m τs bs :
   Forall (type_valid get_env) τs → Forall (byte_valid m) bs →
   type_of <$> flip val_of_bytes bs <$> τs = τs.
-Proof.
-  induction 1; simpl; intros; f_equal; eauto using val_of_bytes_type_of.
-Qed.
+Proof. induction 1; simpl; eauto using val_of_bytes_type_of with f_equal. Qed.
 
 Lemma val_of_bytes_trans m τ bs1 bs2 bs3 :
   type_valid get_env τ → bs1 ⊑@{m}* bs2 → bs2 ⊑@{m}* bs3 →
@@ -645,16 +685,14 @@ Proof.
   * intros τ ? bs1 bs2 bs3 ??. rewrite !val_of_bytes_base.
     intros. f_equal. simplify_equality.
     eauto using bytes_le_resize, base_val_of_bytes_trans.
-  * intros τ n ? IH bs1 bs2 bs3 Hbs1 Hbs2. rewrite !val_of_bytes_array.
-    intros Hbs3. f_equal. simplify_equality.
-    revert bs1 bs2 bs3 Hbs1 Hbs2 Hbs3.
+  * intros τ n ? IH _ bs1 bs2 bs3 Hbs1 Hbs2. rewrite !val_of_bytes_array.
+    intros Hbs3. f_equal. simplify_equality. revert bs1 bs2 bs3 Hbs1 Hbs2 Hbs3.
     induction n; simpl; intros; f_equal; simplify_list_equality;
       eauto using Forall2_drop, Forall2_take.
-  * intros [] s τs Hs Hτs IH bs1 bs2 bs3 Hbs1 Hbs2.
+  * intros [] s τs Hs Hτs IH _ bs1 bs2 bs3 Hbs1 Hbs2.
     { erewrite !val_of_bytes_compound by eauto.
       intros Hbs3. f_equal. simplify_equality.
-      clear Hs Hτs. revert bs1 bs2 bs3 Hbs1 Hbs2 Hbs3.
-      unfold struct_of_bytes.
+      clear Hs Hτs. revert bs1 bs2 bs3 Hbs1 Hbs2 Hbs3. unfold struct_of_bytes.
       induction (struct_fields_same_length τs); simpl in *;
         decompose_Forall; intros; f_equal; simplify_list_equality;
         eauto using Forall2_drop, Forall2_take. }
@@ -663,16 +701,6 @@ Proof.
       intros Hbs3; f_equal; simplify_equality; decompose_Forall; eauto.
     clear Hs Hτs. revert bs1 bs2 bs3 Hbs1 Hbs2 Hbs3.
     induction IH; simpl; intros; f_equal; simplify_list_equality; eauto.
-Qed.
-
-Lemma VUnionNone_typed_alt m s vs τs bs :
-  get_env !! s = Some τs → length τs ≠ 1 →
-  vs = flip val_of_bytes bs <$> τs →
-  Forall (byte_valid m) bs → m ⊢ VUnionNone s vs : TUnion s.
-Proof.
-  intros Hs Hτs_len Hvs Hbs. subst. vtyped_constructor; eauto.
-  elim (env_valid_lookup s τs Hs); simpl;
-    constructor; eauto using val_of_bytes_typed.
 Qed.
 
 Lemma val_freeze_frozen v : val_forall frozen (val_map freeze v).
@@ -693,9 +721,11 @@ Lemma val_freeze_idempotent v :
 Proof. apply val_frozen_freeze, val_freeze_frozen. Qed.
 Lemma val_freeze_type_of v : type_of (val_map freeze v) = type_of v.
 Proof.
-  induction v using val_ind_alt; simpl; simpl; f_equal;
-    auto using base_val_freeze_type_of.
-  by rewrite fmap_length.
+  induction v using val_ind_alt; simpl; simpl; auto.
+   * by rewrite base_val_freeze_type_of.
+   * by match goal with
+     | H: Forall (λ _, type_of _ = _) _ |- _ => destruct H
+     end; simpl; f_equal; rewrite ?fmap_length.
 Qed.
 
 Lemma vals_freeze_frozen vs :
@@ -719,7 +749,7 @@ Proof.
     apply base_val_of_bytes_frozen.
   * intros. rewrite val_of_bytes_array. constructor.
     auto using Forall_array_of_bytes.
-  * intros [] s τs ? _ IH bs.
+  * intros [] s τs ? _ IH _ bs.
     { erewrite val_of_bytes_compound by eauto. constructor.
       auto using Forall_struct_of_bytes. }
     erewrite val_of_bytes_compound by eauto.
@@ -737,15 +767,13 @@ Qed.
 Lemma typed_freeze m v τ : m ⊢ v : τ → m ⊢ val_map freeze v : τ.
 Proof.
   induction 1 using @vtyped_ind; simpl.
-  * constructor. by apply base_typed_freeze.
-  * constructor; auto.
-    + by rewrite fmap_length.
-    + by apply Forall_fmap.
-  * econstructor; eauto. by apply Forall2_fmap_l.
-  * econstructor; eauto.
+  * vtyped_constructor. by apply base_typed_freeze.
+  * vtyped_constructor; auto. by rewrite fmap_length. by apply Forall_fmap.
+  * vtyped_constructor; eauto. by apply Forall2_fmap_l.
+  * vtyped_constructor; eauto.
   * subst. rewrite vals_frozen_freeze by
       eauto using vals_of_bytes_frozen, env_valid_lookup.
-    econstructor; eauto.
+    vtyped_constructor; eauto.
 Qed.
 
 Lemma vtyped_ge m v1 v2 τ : m ⊢ v1 : τ → v1 ⊑@{m} v2 → m ⊢ v2 : τ.
@@ -761,9 +789,8 @@ Proof.
     induction Hvs; intros; decompose_Forall; auto. }
   intros Hv1τ Hv1v2. revert τ Hv1τ. induction Hv1v2 using @val_le_ind;
     intros ? Hv1τ; apply (vtyped_inv_l _ _ _ _ Hv1τ); intros; clear Hv1τ;
-    simplify_map_equality; eauto using VUnionNone_typed_alt;
-    vtyped_constructor; eauto using bytes_valid_ge,
-      Forall2_length, base_typed_ge.
+    simplify_map_equality; vtyped_constructor; eauto using
+      bytes_valid_ge, Forall2_length, base_typed_ge.
 Qed.
 Lemma vtyped_le m v1 v2 τ : m ⊢ v1 : τ → v2 ⊑@{m} v1 → m ⊢ v2 : τ.
 Proof.
@@ -779,10 +806,9 @@ Proof.
   assert (∀ s i τs v1 v2 vs bs,
     get_env !! s = Some τs →
     v1 ⊑@{m} v2 → vs !! i = Some v2 →
-    vs = flip val_of_bytes bs <$> τs →
-    Forall (byte_valid m) bs →
+    vs = flip val_of_bytes bs <$> τs → Forall (byte_valid m) bs →
     (∀ τ, m ⊢ v2 : τ → m ⊢ v1 : τ) →
-    m ⊢ VUnion s i v1 : TUnion s).
+    m ⊢ VUnion s i v1 : union s).
   { intros. subst. edestruct @list_lookup_fmap_inv as [? [??]]; eauto.
     subst. vtyped_constructor; eauto using val_of_bytes_typed,
       env_valid_lookup_lookup. }
@@ -805,13 +831,11 @@ Proof.
     rewrite !val_of_bytes_base, !base_val_of_bytes_resize_take.
     intros. f_equal. simplify_equality. rewrite mask_bytes_take.
     eauto using base_val_of_bytes_masked, Forall_take, Forall2_take.
-  * intros τ n ? IH bs1 bs2 cs2. rewrite !val_of_bytes_array.
-    intros. f_equal. simplify_equality.
-    eauto using array_of_bytes_masked.
-  * intros [] s τs Hs Hτs IH bs1 bs2 cs2.
-    { erewrite !val_of_bytes_compound by eauto.
-      intros ???. f_equal. simplify_equality.
-      eauto using struct_of_bytes_masked. }
+  * intros τ n ? IH _ bs1 bs2 cs2. rewrite !val_of_bytes_array.
+    intros. f_equal. simplify_equality. eauto using array_of_bytes_masked.
+  * intros [] s τs Hs Hτs IH _ bs1 bs2 cs2.
+    { erewrite !val_of_bytes_compound by eauto. intros ???.
+      f_equal. simplify_equality. eauto using struct_of_bytes_masked. }
     erewrite !val_of_bytes_compound by eauto.
     intros. destruct (list_singleton_dec _) as [[??]|_]; subst.
     + simplify_equality. f_equal. rewrite Forall_singleton in IH. eauto.
@@ -842,11 +866,9 @@ Proof.
     { intros ???. apply Forall2_transitive. eauto. }
     assert (∀ s i τs vs2 vs3 v1 v2 bs2 bs3,
       get_env !! s = Some τs → length τs ≠ 1 →
-      vs2 !! i = Some v2 → v1 ⊑@{m} v2 →
-      (∀ v3, v2 ⊑@{m} v3 → v1 ⊑@{m} v3) →
+      vs2 !! i = Some v2 → v1 ⊑@{m} v2 → (∀ v3, v2 ⊑@{m} v3 → v1 ⊑@{m} v3) →
       bs2 ⊑@{m}* bs3 →
-      vs2 = flip val_of_bytes bs2 <$> τs →
-      Forall (byte_valid m) bs2 →
+      vs2 = flip val_of_bytes bs2 <$> τs → Forall (byte_valid m) bs2 →
       vs3 = flip val_of_bytes bs3 <$> τs →
       VUnion s i v1 ⊑@{m} VUnionNone s vs3).
     { intros s i τs ?? v1 v2 bs2 bs3 Hs Hτs Hv2 ??????. subst.
@@ -868,8 +890,7 @@ Proof.
     intros v1 v2 v3 Hv1v2. revert v3. induction Hv1v2 using @val_le_ind;
       intros ? Hv2v3; apply (val_le_inv_l _ _ _ _ Hv2v3); intros;
       simplify_map_equality; first
-       [ by eauto
-       | val_le_constructor; eauto; etransitivity; eauto ].
+       [ by eauto | val_le_constructor; eauto; etransitivity; eauto ].
   * assert (∀ vs1 vs2,
       Forall2 (λ v1 v2, v2 ⊑@{m} v1 → v1 = v2) vs1 vs2 →
       vs2 ⊑@{m}* vs1 → vs1 = vs2).
@@ -880,9 +901,8 @@ Proof.
       bs1 ⊑@{m}* bs2 →
       vs2 = flip val_of_bytes bs1 <$> τs → Forall (byte_valid m) bs1 →
       vs1 = flip val_of_bytes bs2 <$> τs → vs1 = vs2).
-    { intros ?? τs ?? Hτs ?????. subst.
-      induction Hτs; simpl in *; decompose_Forall;
-        f_equal; eauto using val_of_bytes_le. }
+    { intros ?? τs ?? Hτs ?????. subst. induction Hτs; simpl in *;
+        decompose_Forall; f_equal; eauto using val_of_bytes_le. }
     induction 1 using @val_le_ind;
       intros Hv2v1; apply (val_le_inv _ _ _ _ Hv2v1); intros;
       f_equal; eauto using env_valid_lookup;
@@ -922,9 +942,7 @@ Lemma mval_to_val_typed m w τ : m ⊢ w : τ → m ⊢ mval_to_val w : τ.
 Proof.
   induction 1 using @mtyped_ind; simpl.
   * vtyped_constructor. eauto using base_val_of_bytes_typed.
-  * vtyped_constructor; trivial.
-    + by rewrite fmap_length.
-    + by apply Forall_fmap.
+  * vtyped_constructor; trivial. by rewrite fmap_length. by apply Forall_fmap.
   * vtyped_constructor; eauto. by apply Forall2_fmap_l.
   * vtyped_constructor; eauto.
   * eapply val_of_bytes_typed; eauto. constructor; eauto.
@@ -948,13 +966,11 @@ Lemma mval_to_val_union_free_2 m w τ :
 Proof.
   assert (∀ ws,
     Forall (λ w, munion_free w → union_free (mval_to_val w)) ws →
-    Forall munion_free ws →
-    Forall union_free (mval_to_val <$> ws)).
+    Forall munion_free ws → Forall union_free (mval_to_val <$> ws)).
   { induction 1; simpl; intros; decompose_Forall; auto. }
   assert (∀ ws τs,
     Forall2 (λ w _, munion_free w → union_free (mval_to_val w)) ws τs →
-    Forall munion_free ws →
-    Forall union_free (mval_to_val <$> ws)).
+    Forall munion_free ws → Forall union_free (mval_to_val <$> ws)).
   { induction 1; simpl; intros; decompose_Forall; auto. }
   induction 1 using @mtyped_ind; simpl.
   * constructor.
@@ -976,7 +992,7 @@ Proof.
   * intros τ ? bs. by rewrite mval_of_bytes_base, val_of_bytes_base.
   * intros. rewrite mval_of_bytes_array, val_of_bytes_array.
     simpl. erewrite array_of_bytes_fmap; eauto.
-  * intros [] s τs Hs Hτs IH bs.
+  * intros [] s τs Hs Hτs IH _ bs.
     { erewrite mval_of_bytes_compound, val_of_bytes_compound by eauto.
       simpl. erewrite struct_of_bytes_fmap; eauto. }
     erewrite mval_of_bytes_compound, val_of_bytes_compound by eauto.
@@ -1024,7 +1040,7 @@ Proof.
     m ⊢ w1 : τ →
     (∀ w2, w1 ⊑@{m} w2 → mval_to_val w1 ⊑@{m} mval_to_val w2) →
     length τs ≠ 1 →
-    resize (size_of (TUnion s)) BUndef (mval_to_bytes w1) ⊑@{m}* bs →
+    resize (size_of (union s)) BUndef (mval_to_bytes w1) ⊑@{m}* bs →
     VUnion s i (mval_to_val w1) ⊑@{m}
       VUnionNone s (flip val_of_bytes bs <$> τs)).
   { intros s i τs w1 τ bs Hs Hi Hw1τ IH Hτs_len Hbs.
@@ -1072,7 +1088,7 @@ Proof.
   + intros. decompose_elem_of. apply Forall_replicate, BUndef_valid.
   + unfold compose. simpl.
     induction Hvs; constructor; intros; decompose_elem_of;
-       eauto using Forall_resize, BUndef_valid, mval_to_bytes_valid.
+      eauto using Forall_resize, BUndef_valid, mval_to_bytes_valid.
   + eauto using bytes_valid_ge, bytes_join_Some_l.
 Qed.
 
@@ -1080,13 +1096,12 @@ Lemma mval_of_val_typed m v τ w : m ⊢ v : τ → w ∈ mval_of_val v → m �
 Proof.
   intros Hvτ. revert v τ Hvτ w. refine (vtyped_ind _ _ _ _ _ _ _); simpl.
   * intros. decompose_elem_of. erewrite type_of_correct by eauto.
-    mtyped_constructor; eauto using
-      base_typed_type_valid, base_val_to_bytes_valid,
-      base_val_to_bytes_length_typed.
+    mtyped_constructor; eauto using base_typed_type_valid,
+      base_val_to_bytes_valid, base_val_to_bytes_length_typed.
   * intros. decompose_elem_of. mtyped_constructor.
-    + done.
-    + subst. by erewrite <-mapM_length by eauto.
+    + symmetry. eapply mapM_length; eauto.
     + eapply elem_of_mapM_Forall; eauto.
+    + done. 
   * intros. decompose_elem_of. mtyped_constructor; eauto.
     eapply elem_of_mapM_Forall2_l; eauto.
   * intros. decompose_elem_of. mtyped_constructor; eauto.
@@ -1095,21 +1110,28 @@ Proof.
     econstructor; eauto using union_to_bytes_valid_aux, union_to_bytes_length.
 Qed.
 
-Lemma union_to_bytes_valid m sz vs τs bs :
+Lemma val_of_bytes_union_to_bytes m sz vs τs bs :
+  m ⊢* vs :* τs →
   bs ∈ union_to_bytes mval_of_val sz vs →
-  m ⊢* vs :* τs → Forall (byte_valid m) bs.
+  flip val_of_bytes bs <$> τs = vs.
 Proof.
-  intros Hbs Hvs. revert Hbs. apply union_to_bytes_valid_aux with τs.
+  intros Hvs. unfold union_to_bytes. rewrite elem_of_filter.
+  erewrite list_fmap_compose, fmap_type_of by eauto. by intros [??].
+Qed.
+Lemma union_to_bytes_valid m sz vs τs bs :
+  m ⊢* vs :* τs →
+  bs ∈ union_to_bytes mval_of_val sz vs → Forall (byte_valid m) bs.
+Proof.
+  intros Hvs. apply union_to_bytes_valid_aux with τs.
   induction Hvs; constructor; eauto using mval_of_val_typed.
 Qed.
 
 Lemma mval_of_to_val m v τ w :
   m ⊢ v : τ → w ∈ mval_of_val v → val_map freeze v = mval_to_val w.
 Proof.
-  intros Hvτ. revert v τ Hvτ w.
-  refine (vtyped_ind _ _ _ _ _ _ _); simpl.
+  intros Hvτ. revert v τ Hvτ w. refine (vtyped_ind _ _ _ _ _ _ _); simpl.
   * intros. decompose_elem_of. simpl. by rewrite base_val_of_to_bytes.
-  * intros vs τ n Hτ Hn _ IH w Hw.
+  * intros vs τ Hvs IH _ w Hw.
     rewrite elem_of_fmap in Hw. destruct Hw as (ws & ? & Hws); subst.
     simpl. f_equal. rewrite elem_of_mapM in Hws.
     induction Hws; simpl; decompose_Forall; f_equal; auto.
@@ -1122,18 +1144,16 @@ Proof.
     rewrite elem_of_fmap in Hw. destruct Hw as (cs & ? & Hcs); subst.
     simpl. erewrite val_of_bytes_compound by eauto.
     destruct (list_singleton_dec _) as [[??]|_]; subst; [done|].
-    f_equal. unfold union_to_bytes in Hcs.
-    rewrite elem_of_filter in Hcs. destruct Hcs as [Hcs _].
-    erewrite Hcs, list_fmap_compose, fmap_type_of by eauto.
-    by rewrite vals_frozen_freeze by
+    f_equal. rewrite vals_frozen_freeze by
       eauto using vals_of_bytes_frozen, env_valid_lookup.
+    symmetry. eauto using val_of_bytes_union_to_bytes.
 Qed.
 
 Lemma val_of_to_bytes_union_free m v τ bs :
   m ⊢ v : τ → union_free v →
   bs ∈ mval_to_bytes <$> mval_of_val v → val_of_bytes τ bs = val_map freeze v.
 Proof.
-  intros Hvτ ? Hbs. apply elem_of_fmap in Hbs. destruct Hbs as (w & ? & Hw).
+  intros Hvτ ? Hbs. apply elem_of_fmap in Hbs. destruct Hbs as (w&?&Hw).
   assert (m ⊢ w : τ) by eauto using mval_of_val_typed.
   eapply mval_of_to_val in Hw; eauto. subst.
   rewrite <-!mval_of_bytes_to_val by eauto using vtyped_type_valid.
@@ -1141,18 +1161,16 @@ Proof.
   apply mval_to_val_union_free_1. rewrite <-Hw. by apply union_free_freeze.
 Qed.
 
-Lemma union_to_of_bytes_exists_help m τs sz bs2 :
-  let vs := flip val_of_bytes bs2 <$> τs in
-  Forall (type_valid get_env) τs →
-  Forall (λ τ, size_of τ ≤ sz) τs →
-  Forall (byte_valid m) bs2 →
-  Forall (λ τ, ∀ bs2, Forall (byte_valid m) bs2 →
+Lemma union_to_of_bytes_exists_help m τs sz bs2
+    (vs := flip val_of_bytes bs2 <$> τs) :
+  Forall (type_valid get_env) τs → Forall (λ τ, size_of τ ≤ sz) τs →
+  Forall (byte_valid m) bs2 → Forall (λ τ, ∀ bs2, Forall (byte_valid m) bs2 →
     ∃ bs1, bs1 ∈ mval_to_bytes <$> mval_of_val (val_of_bytes τ bs2) ∧
       bs1 ⊑@{m}* resize (size_of τ) BUndef bs2) τs →
   ∃ bs1, bs1 ∈ union_to_bytes mval_of_val sz vs ∧
     bs1 ⊑@{m}* resize sz BUndef bs2.
 Proof.
-  intros vs Hτs Hsz Hbs2 IH. cut (∃ bs1,
+  intros Hτs Hsz Hbs2 IH. cut (∃ bs1,
     flip val_of_bytes bs1 <$> τs = flip val_of_bytes bs2 <$> τs ∧
     bs1 ∈ intersection_with_list bytes_join {[ replicate sz BUndef ]} $
       fmap (resize sz BUndef ∘ mval_to_bytes) ∘ mval_of_val <$> vs ∧
@@ -1163,8 +1181,7 @@ Proof.
     elim Hτs; simpl; constructor; auto using val_of_bytes_typed. }
   unfold vs. clear vs. revert bs2 Hbs2.
   induction IH as [|τ τs IHτ _ IHτs]; intros bs2 Hbs2; simpl.
-  { eexists (replicate sz BUndef).
-    rewrite elem_of_singleton. split_ands; auto.
+  { eexists (replicate sz BUndef). rewrite elem_of_singleton. split_ands; auto.
     eapply Forall2_replicate_l; eauto using resize_length.
     eapply Forall_resize; eauto. eapply Forall_impl; eauto. by constructor. }
   rewrite Forall_cons in Hτs. destruct Hτs as [Hτ Hτs].
@@ -1176,7 +1193,7 @@ Proof.
   destruct (IHτs Hτs Hsz' bs2) as (bs4 & ? & Hbs4 & ?); trivial.
   assert (Forall (byte_valid m) bs4).
   { apply (union_to_bytes_valid m sz (flip val_of_bytes bs2 <$> τs) τs);
-      eauto using Forall_val_of_bytes_typed.
+      eauto using fmap_val_of_bytes_typed.
     unfold union_to_bytes. apply elem_of_filter. split; auto.
     rewrite list_fmap_compose, (val_of_bytes_fmap_type_of m); eauto. }
   destruct (bytes_join_exists m (resize sz BUndef bs3) bs4
@@ -1206,16 +1223,14 @@ Lemma val_to_of_bytes_exists m τ bs2 :
   ∃ bs1, bs1 ∈ mval_to_bytes <$> mval_of_val (val_of_bytes τ bs2) ∧
     bs1 ⊑@{m}* resize (size_of τ) BUndef bs2.
 Proof.
-  intros Hvτ. revert τ Hvτ bs2.
-  refine (type_env_ind _ _ _ _).
+  intros Hvτ. revert τ Hvτ bs2. refine (type_env_ind _ _ _ _).
   * intros τ ? bs2 Hbs2. destruct (base_val_to_of_bytes_le m τ
-      (resize (size_of (TBase τ)) BUndef bs2)) as (bs1 & ? & ?).
+      (resize (size_of (base τ)) BUndef bs2)) as (bs1 & ? & ?).
     { eauto using Forall_resize, BUndef_valid. }
     { by rewrite resize_length. }
-    exists bs1. split; [|done].
-    rewrite val_of_bytes_base. simpl. rewrite <-collection_fmap_compose.
-    apply elem_of_fmap. by exists bs1.
-  * intros τ n Hτ IH bs2 Hbs2. rewrite val_of_bytes_array. simpl.
+    exists bs1. split; [|done]. rewrite val_of_bytes_base. simpl.
+    rewrite <-collection_fmap_compose. apply elem_of_fmap. by exists bs1.
+  * intros τ n Hτ IH _ bs2 Hbs2. rewrite val_of_bytes_array. simpl.
     simpl. setoid_rewrite <-collection_fmap_compose.
     unfold compose. simpl. rewrite size_of_array.
     revert bs2 Hbs2. induction n as [|n IHn]; intros bs2 Hbs2; simpl.
@@ -1230,7 +1245,7 @@ Proof.
     { simpl. by f_equal. }
     rewrite elem_of_bind. exists v. split; [|done].
     rewrite elem_of_bind. exists vs. split; [by left|done].
-  * intros [] s τs Hs Hτs IH bs2 Hbs2.
+  * intros [] s τs Hs Hτs IH _ bs2 Hbs2.
     { erewrite val_of_bytes_compound by eauto.
       simpl. setoid_rewrite <-collection_fmap_compose.
       unfold compose. simpl. erewrite size_of_struct by eauto.
@@ -1257,20 +1272,18 @@ Proof.
       setoid_rewrite <-collection_fmap_compose. unfold compose. simpl.
       destruct (IH bs2) as (bs3 & Hbs3 & ?); trivial.
       apply elem_of_fmap in Hbs3. destruct Hbs3 as (v & ? & ?).
-      exists (resize (size_of (TUnion s)) BUndef bs3).
+      exists (resize (size_of (union s)) BUndef bs3).
       split; [| eauto using Forall2_resize_ge_r, BUndef_le,
         Forall_BUndef_le, size_of_union_singleton].
       apply elem_of_fmap. subst. by exists v. }
-    destruct (union_to_of_bytes_exists_help m τs (size_of (TUnion s)) bs2)
+    destruct (union_to_of_bytes_exists_help m τs (size_of (union s)) bs2)
       as (bs1 & ? & ?); eauto using size_of_union.
     exists bs1. split; [|done]. simpl. setoid_rewrite <-collection_fmap_compose.
     apply elem_of_fmap. by exists bs1.
 Qed.
 
-Lemma union_to_of_bytes_exists m τs sz bs2 :
-  let vs := flip val_of_bytes bs2 <$> τs in
-  Forall (type_valid get_env) τs →
-  Forall (λ τ, size_of τ ≤ sz) τs →
+Lemma union_to_of_bytes_exists m τs sz bs2 (vs:=flip val_of_bytes bs2 <$> τs) :
+  Forall (type_valid get_env) τs → Forall (λ τ, size_of τ ≤ sz) τs →
   Forall (byte_valid m) bs2 →
   ∃ bs1, bs1 ∈ union_to_bytes mval_of_val sz vs ∧
     bs1 ⊑@{m}* resize sz BUndef bs2.
@@ -1284,17 +1297,17 @@ Proof.
   revert v τ. refine (vtyped_ind _ _ _ _ _ _ _); simpl.
   * intros v τ Hvτ. destruct (base_val_to_bytes_exists v) as [bs ?].
     exists (MBase τ bs). erewrite type_of_correct by eauto. esolve_elem_of.
-  * intros vs τ n Hτ ? Hvs IH. subst.
+  * intros vs τ Hvs IH _. subst.
     assert (∃ ws, ws ∈ mapM mval_of_val vs) as [ws ?].
     { clear Hvs. induction IH; esolve_elem_of. }
-    exists (MArray τ ws). esolve_elem_of.
+    exists (MArray ws). esolve_elem_of.
   * intros s vs τs Hs Hτs IH.
     assert (∃ ws, ws ∈ mapM mval_of_val vs) as [ws ?].
     { clear Hs Hτs. induction IH; esolve_elem_of. }
     exists (MStruct s ws). esolve_elem_of.
   * intros s i τs v τ Hs Hτs ? [w Hw]. exists (MUnion s i w). esolve_elem_of.
   * intros s vs τs bs Hs Hτs ??? Hbs.
-    destruct (union_to_of_bytes_exists m τs (size_of (TUnion s)) bs)
+    destruct (union_to_of_bytes_exists m τs (size_of (union s)) bs)
       as (bs' & ? & Hbs'); eauto using size_of_union, env_valid_lookup.
     exists (MUnionNone s bs'). esolve_elem_of.
 Qed.
@@ -1304,23 +1317,22 @@ Lemma mval_of_to_val_exists m w τ :
 Proof.
   revert w τ. refine (mtyped_ind _ _ _ _ _ _ _); simpl.
   * intros τ bs ???.
-    destruct (base_val_to_of_bytes_le m τ bs) as (bs' & ? & ?); trivial.
+    destruct (base_val_to_of_bytes_le m τ bs) as (bs'&?&?); trivial.
     exists (MBase τ bs'). rewrite base_val_of_bytes_type_of by done.
     split. esolve_elem_of. by constructor.
-  * intros ws τ n Hτ ? Hws IH. subst.
+  * intros ws τ Hws IH _. subst.
     assert (∃ ws', ws' ∈ mapM mval_of_val (mval_to_val <$> ws) ∧
-      ws' ⊑@{m}* ws) as (ws' & ? & ?).
-    { clear Hws. induction IH; esolve_elem_of. }
-    exists (MArray τ ws'). split. esolve_elem_of. by constructor.
+      ws' ⊑@{m}* ws) as (ws'&?&?). by (clear Hws; induction IH; esolve_elem_of).
+    exists (MArray ws'). split. esolve_elem_of. by constructor.
   * intros s ws τs Hs Hτs IH.
     assert (∃ ws', ws' ∈ mapM mval_of_val (mval_to_val <$> ws) ∧
-      ws' ⊑@{m}* ws) as (ws' & ? & ?).
+      ws' ⊑@{m}* ws) as (ws'&?&?).
     { clear Hs Hτs. induction IH; esolve_elem_of. }
     exists (MStruct s ws'). split. esolve_elem_of. by constructor.
   * intros s i τs w τ Hs Hτs ? (w' & ? & ?).
     exists (MUnion s i w'). split. esolve_elem_of. by constructor.
   * intros s τs bs Hs Hτs Hbs Hlen.
-    destruct (union_to_of_bytes_exists m τs (size_of (TUnion s)) bs)
+    destruct (union_to_of_bytes_exists m τs (size_of (union s)) bs)
      as (bs' & Hbs' & Hbs'bs); eauto using size_of_union, env_valid_lookup.
     rewrite resize_all_alt in Hbs'bs by done.
     exists (MUnionNone s bs'). erewrite val_of_bytes_compound by eauto.
@@ -1350,18 +1362,17 @@ Proof.
     exists (MBase τ bs1). subst. simpl.
     erewrite !type_of_correct by eauto using base_typed_ge.
     split; [esolve_elem_of|]. by constructor.
-  * intros vs1 vs2 τ _ IH τ' Hτ'. apply (vtyped_inv_l _ _ _ _ Hτ').
-    clear τ' Hτ'. intros n Hτ Hn Hvs1 w2 Hw2. simpl in *.
+  * intros vs1 vs2 Hvs IH τ' Hτ'. apply (vtyped_inv_l _ _ _ _ Hτ').
+    clear τ' Hτ'. intros τ ?? Hvs1 _ w2 Hw2; subst. simpl in *.
     apply elem_of_fmap in Hw2. destruct Hw2 as (ws2 & ? & Hws2). subst.
     apply elem_of_mapM in Hws2. assert (∃ ws1,
       Forall2 (λ w1 v1, w1 ∈ mval_of_val v1) ws1 vs1 ∧
       ws1 ⊑@{m}* ws2) as (ws1 & ? & ?).
     { revert ws2 Hws2. induction IH; intros; decompose_Forall; naive_solver. }
-    exists (MArray τ ws1); split; [|by constructor].
+    exists (MArray ws1); split; [|by constructor].
     apply elem_of_fmap. exists ws1. by rewrite elem_of_mapM.
-  * intros s vs1 vs2 _ IH τ' Hτ'.
-    apply (vtyped_inv_l _ _ _ _ Hτ'). clear τ' Hτ'.
-    intros τs _ Hvs1 w2 Hw2. simpl in *.
+  * intros s vs1 vs2 _ IH τ' Hτ'. apply (vtyped_inv_l _ _ _ _ Hτ').
+    clear τ' Hτ'. intros τs _ Hvs1 w2 Hw2. simpl in *.
     apply elem_of_fmap in Hw2. destruct Hw2 as (ws2 & ? & Hws2).
     subst. apply elem_of_mapM in Hws2. assert (∃ ws1,
       Forall2 (λ w1 v1, w1 ∈ mval_of_val v1) ws1 vs1 ∧
@@ -1380,18 +1391,18 @@ Proof.
     apply (vtyped_inv_l _ _ _ _ Hτ').
     clear τ' Hτ'. intros ??????? w2 Hw2. simplify_option_equality.
     apply elem_of_fmap in Hw2. destruct Hw2 as (bs4 & ? & Hbs4). subst.
-    assert (length bs4 = size_of (TUnion s))
+    assert (length bs4 = size_of (union s))
       by eauto using union_to_bytes_length.
     assert (Forall (byte_valid m) bs4).
-    { eapply union_to_bytes_valid; eauto using
-        Forall_val_of_bytes_typed, bytes_valid_ge, env_valid_lookup. }
+    { eapply union_to_bytes_valid with _ (flip val_of_bytes bs2 <$> τs) _;
+        eauto using fmap_val_of_bytes_typed, bytes_valid_ge, env_valid_lookup. }
     unfold union_to_bytes in Hbs4.
     apply elem_of_filter in Hbs4. destruct Hbs4 as (Hbs2 & ?).
     rewrite list_fmap_compose, (val_of_bytes_fmap_type_of m) in Hbs2
       by eauto using env_valid_lookup, bytes_valid_ge.
     rewrite <-(Forall_val_of_bytes_masked m τs bs1 bs2 bs4)
       by eauto using env_valid_lookup.
-    destruct (union_to_of_bytes_exists m τs (size_of (TUnion s))
+    destruct (union_to_of_bytes_exists m τs (size_of (union s))
       (mask_bytes bs1 bs4)) as (bs3 & Hbs3 & Hbs3bs4);
       eauto using size_of_union, env_valid_lookup, mask_bytes_valid.
     exists (MUnionNone s bs3). split; [esolve_elem_of |].
@@ -1402,30 +1413,70 @@ Proof.
     apply (vtyped_inv_l _ _ _ _ Hτ'). clear τ' Hτ'.
     intros ? τ ? Hiτ Hv1τ w2' Hw2'. simplify_option_equality.
     apply elem_of_fmap in Hw2'. destruct Hw2' as (bs3 & Hv2 & Hbs3).
-    assert (length bs3 = size_of (TUnion s))
+    assert (length bs3 = size_of (union s))
       by eauto using union_to_bytes_length.
     unfold union_to_bytes in Hbs3.
     assert (Forall (byte_valid m) bs3).
-    { eapply union_to_bytes_valid; eauto using
-        Forall_val_of_bytes_typed, env_valid_lookup. }
+    { eapply union_to_bytes_valid with _ (flip val_of_bytes bs2 <$> τs) _;
+        eauto using fmap_val_of_bytes_typed, env_valid_lookup. }
     apply elem_of_filter in Hbs3. destruct Hbs3 as [Hbs3 ?].
     destruct (val_to_of_bytes_exists m τ bs3) as (bs1 & Hbs1 & ?);
       eauto using env_valid_lookup_lookup.
     rewrite list_fmap_compose, (val_of_bytes_fmap_type_of m) in Hbs3
       by eauto using env_valid_lookup.
-    apply (f_equal (!! i)) in Hbs3.
-    rewrite !list_lookup_fmap, Hiτ in Hbs3.
+    apply (f_equal (!! i)) in Hbs3. rewrite !list_lookup_fmap, Hiτ in Hbs3.
     rewrite !list_lookup_fmap, Hiτ in Hi.
     rewrite elem_of_fmap in Hbs1. destruct Hbs1 as (w2 & ? & Hw2).
     simplify_option_equality.
     destruct (IH τ Hv1τ w2) as (w1 & ? & ?); [by rewrite Hbs3|].
     exists (MUnion s i w1). split; [esolve_elem_of |].
     econstructor; eauto using mval_of_val_typed.
-    transitivity (resize (size_of (TUnion s)) BUndef (mval_to_bytes w2));
+    transitivity (resize (size_of (union s)) BUndef (mval_to_bytes w2));
       eauto using bytes_le_resize, mval_to_bytes_le.
-    rewrite <-(resize_all_alt bs3 (size_of (TUnion s)) BUndef) by done.
+    rewrite <-(resize_all_alt bs3 (size_of (union s)) BUndef) by done.
     eauto using Forall2_resize_ge_r, BUndef_le, Forall_BUndef_le,
       size_of_union_lookup.
+Qed.
+
+Global Instance: TypeCheckSpec M (type Ti) (val Ti Vi).
+Proof.
+  intros m. assert (∀ vs τs,
+    Forall (λ v, ∀ τ, vtype_check m v = Some τ → m ⊢ v : τ) vs →
+    Forall2 (λ v τ, vtype_check m v = Some τ) vs τs → m ⊢* vs :* τs).
+  { induction 2; intros; decompose_Forall; subst; eauto. }
+  assert (∀ vs τ,
+    m ⊢* vs : τ → Forall (λ v, vtype_check m v = Some τ) vs →
+    mapM (type_check m) vs = Some (replicate (length vs) τ)).
+  { intros. apply mapM_Some, Forall2_replicate_r; decompose_Forall; eauto. }
+  assert (∀ sz vs τs bs,
+    choose (union_to_bytes mval_of_val sz vs) = Some bs →
+    bs ∈ union_to_bytes mval_of_val sz vs).
+  { intros. by apply choose_Some. }
+  assert (∀ s τs bs,
+    get_env !! s = Some τs → Forall (byte_valid m) bs →
+    choose (union_to_bytes mval_of_val (size_of (union s))
+      (flip val_of_bytes bs <$> τs)) ≠ None).
+  { intros s τs bs ??. rewrite not_eq_None_Some.
+    rewrite <-choose_is_Some, not_elem_of_equiv_empty.
+    destruct (union_to_of_bytes_exists m τs (size_of (union s))  bs) as (?&?&?);
+      eauto using size_of_union, env_valid_lookup. }
+  intros v τ. unfold type_check. split.
+  * revert τ. induction v using @val_ind_alt; intros; simplify_option_equality.
+    + vtyped_constructor; eauto. by apply type_check_sound.
+    + case_match; simplify_option_equality.
+      vtyped_constructor; eauto. eapply Forall2_Forall_typed; eauto.
+    + vtyped_constructor; decompose_Forall; eauto.
+    + vtyped_constructor; eauto.
+    + vtyped_constructor; eauto using
+        val_of_bytes_union_to_bytes, eq_sym, union_to_bytes_valid.
+  * induction 1 using @vtyped_ind; simplify_option_equality.
+    + by erewrite type_check_complete by eauto.
+    + decompose_Forall_hyps; simplify_option_equality; try done;
+        exfalso; eauto using Forall_replicate_eq.
+    + erewrite mapM_Some_2; eauto. by simplify_option_equality.
+    + done.
+    + erewrite mapM_Some_2; eauto; simplify_option_equality.
+      destruct (choose _) eqn:?; naive_solver.
 Qed.
 
 Lemma val_lookup_nil v : v !! [] = Some v.
@@ -1463,20 +1514,17 @@ Lemma mval_of_val_lookup_seg m w1 τ rs v1 :
   m ⊢ w1 : τ → mval_to_val w1 !! rs = Some v1 →
   ∃ w2, w1 !! rs = Some w2 ∧ mval_to_val w2 = v1.
 Proof.
-  destruct 1 using @mtyped_case; destruct rs; intros; simplify_option_equality.
-  * rewrite list_lookup_fmap in H7. simplify_option_equality. eauto.
-  * exfalso; eauto using fmap_length.
-  * rewrite list_lookup_fmap in H6. simplify_option_equality. eauto.
-  * eauto.
-  * erewrite val_of_bytes_compound in H8 by eauto.
-    by destruct (list_singleton_dec _) as [[??]|?].
-  * erewrite val_of_bytes_compound in H8 by eauto.
-    by destruct (list_singleton_dec _) as [[??]|?].
-  * erewrite val_of_bytes_compound in H8 by eauto.
-    destruct (list_singleton_dec _) as [[??]|?]; simplify_option_equality.
-    rewrite list_lookup_fmap in H8. simplify_option_equality.
-    rewrite mval_of_bytes_take by eauto using env_valid_lookup_lookup.
-    rewrite <-mval_of_bytes_to_val by eauto using env_valid_lookup_lookup. eauto.
+  destruct 1 using @mtyped_case; destruct rs; intros;
+    repeat match goal with
+    | _ => progress simplify_option_equality
+    | H: (_ <$> _) !! _ = Some _ |- _ => rewrite list_lookup_fmap in H
+    | H: length (_ <$> _) ≠ _ |- _ => rewrite fmap_length in H
+    | H: val_of_bytes _ _ !! _ = Some _ |- _ =>
+      erewrite val_of_bytes_compound in H by eauto;
+      destruct (list_singleton_dec _) as [[??]|?]
+    end; eauto.
+  rewrite mval_of_bytes_take, <-mval_of_bytes_to_val;
+    eauto using env_valid_lookup_lookup.
 Qed.
 
 Lemma val_lookup_seg_Some m v τ rs v' :
